xtactics.md
@@ -1,0 +1,23 @@
+# Tactics to deal with ntriple/nwp
+
+1. `LibSepReference.v`:
+  - `xfocus l` : focuses on the `l`'s component
+  - `xunfocus` : unfocuses the focused component 
+  - `xin l : tac` : `xfocus l; tac; xunfocus` + some clean up (recommended to use instead `xfocus`/`xunfocus`)
+  - `xfocus l P` : focuses on the parts of `l`'s component that satisfies `P`
+  - `xframe H` : frames out `H` form the precondition if the post condition has form `Q \* \Top`
+  - `xnsimpl` : `xsimpl` for `ntriples` (use only if `xsimpl` fails)
+
+2. `Loops.v`:
+  - `xfor_sum Inv R R' op s` : applies `xfor_big_op_lemma` lemma with corresponded arguments. This tactic is applicable for goals of the form:
+  ```
+  {{ H }}
+  [{
+    [i: ld in `{_} => for i <- [0, N] { C1 }; C2]
+    [j: ld in S    => C3]
+  }]
+  {{ Q }}
+  ```
+     
+
+Enjoy!!
